src/demo/flasher/NotAutomat.thy
@@ -21,11 +21,30 @@ abbreviation notStep::"(S_not \<Rightarrow> (inNot\<^sup>\<Omega> \<rightarrow> 
 "notStep \<equiv> dawStateSem dAnot"
 
 definition notSpf::"(inNot\<^sup>\<Omega> \<rightarrow> outNot\<^sup>\<Omega>)"where
-"notSpf = notStep (dawInitState dAnot)"
+"notSpf = dasSem dAnot"
 
 
-interpretation not_sscanl:smapGen "dAnot" "buildNotinSBE" "buildNotoutSBE" Single
+interpretation not_smap:smapGen "dAnot" "buildNotinSBE" "buildNotoutSBE" Single
   sorry
 
+lemma notingetset_eq:"notInSBE.getterSB\<cdot>(notInSBE.setterSB\<cdot>s) = s"
+  by(simp add: notInSBE.getset_eq)
+
+lemma notoutgetset_eq:"notOutSBE.getterSB\<cdot> (notOutSBE.setterSB\<cdot>s) = s"
+  by(simp add: notOutSBE.getset_eq)
+
+lemma notstep2smap:"notOutSBE.getterSB\<cdot>(notStep state\<cdot>(notInSBE.setterSB\<cdot>input)) = (smap not_smap.smapTransition)\<cdot>input"
+  by (simp add: notInSBE.getset_eq not_smap.daut2smap notoutgetset_eq)
+
+thm dAutomaton_weak.select_convs
+
+lemma "notOutSBE.getterSB\<cdot>(notSpf\<cdot>(notInSBE.setterSB\<cdot>input)) = \<up>True \<bullet>(smap not_smap.smapTransition)\<cdot>input"
+  apply(simp add: notSpf_def dasSem_def)
+  apply(subst notOutSBE.gettersb_unfold)
+  apply(simp add: dAnot_def)
+  by (metis dAnot_def dAutomaton_weak.select_convs(1) notstep2smap)
+
+lemma "smap not_smap.smapTransition\<cdot>(\<up>bool \<bullet> s) = \<up>(\<not>bool) \<bullet> smap not_smap.smapTransition\<cdot>s"
+  by(simp add: dAnot_def dNot_transition_def)
 
 end
