src/demo/flasher/Flasher.thy
@@ -6,9 +6,10 @@ begin
 (*Composition of And and Not SPFs*)
 
 definition flasherComp::"((inAnd\<union>inNot) - (outAnd \<union> outNot))\<^sup>\<Omega> \<rightarrow>(outAnd \<union> outNot)\<^sup>\<Omega>"where
-"flasherComp = genComp\<cdot>andSpf\<cdot>notSpf"
+"flasherComp = andSpf \<otimes> notSpf"
 
 lemma flasherhd:"\<exists>rest. flasherComp\<cdot>(sbe \<bullet>\<^sup>\<surd> sb) = sbeConvert(sbeGen.setter buildAndoutSBE (True \<and> sbeGen.getter buildNotinSBE (sbeConvert sbe)))\<bullet>\<^sup>\<surd> rest"
+
   sorry
 
 
