src/spf/SPFcomp.thy
@@ -13,10 +13,8 @@ definition genComp :: "('I1\<^sup>\<Omega> \<rightarrow> 'O1\<^sup>\<Omega>) \<r
 "genComp \<equiv> \<Lambda> spf1 spf2 sbIn . fix\<cdot>(\<Lambda> sbOut. spf1\<cdot>(sbIn \<uplus>\<^sub>\<star> sbOut) \<uplus>\<^sub>\<star> spf2\<cdot>(sbIn \<uplus>\<^sub>\<star> sbOut))"
 
 subsection \<open>General composition abbreviation\<close>
- (* inifxr \<otimes> ... without magic
+ (* inifxr \<otimes> ... without magic*)
 abbreviation genComp_abbr :: "('I1\<^sup>\<Omega> \<rightarrow> 'O1\<^sup>\<Omega>) \<Rightarrow> ('I2\<^sup>\<Omega> \<rightarrow> 'O2\<^sup>\<Omega>) \<Rightarrow> ((('I1 \<union> 'I2) - ('O1 \<union> 'O2))\<^sup>\<Omega> \<rightarrow> ('O1 \<union> 'O2)\<^sup>\<Omega>)" (infixr "\<otimes>" 70) where 
 "spf1 \<otimes> spf2 \<equiv> genComp\<cdot>spf1\<cdot>spf2"
-*)
-
 
 end
